block 1, 2, 3, 4

Coq/Cln/Cln_SupportAlgebra.v
@@ -134,13 +134,139 @@ Require Import Cln_Grade.
 Require Import Cln_BoolDist.
 
 From Coq Require Import List QArith.
+From Coq Require Import Lia.
+Require Import Coq.Program.Equality.
 
-        (* Support cardinality *)
+Import ListNotations.
+
+(* ------------------------------------------------------------------ *)
+(* Small list helpers (avoid depending on library lemma names)         *)
+(* ------------------------------------------------------------------ *)
+
+Lemma length_filter_le :
+  forall (A : Type) (p : A -> bool) (l : list A),
+    (length (filter p l) <= length l)%nat.
+Proof.
+  intros A p l; induction l as [|a tl IH]; simpl; auto.
+  destruct (p a); simpl; lia.
+Qed.
+
+Lemma NoDup_filter :
+  forall (A : Type) (p : A -> bool) (l : list A),
+    NoDup l -> NoDup (filter p l).
+Proof.
+  intros A p l Hnd.
+  induction Hnd as [|a tl Hnotin Hnd IH]; simpl.
+  - constructor.
+  - destruct (p a) eqn:Ha.
+    + constructor.
+      * intro Hin.
+        apply filter_In in Hin as [Hin _].
+        contradiction.
+      * exact IH.
+    + exact IH.
+Qed.
+
+Lemma NoDup_incl_length :
+  forall (A : Type) (l1 l2 : list A),
+    NoDup l1 -> incl l1 l2 -> (length l1 <= length l2)%nat.
+Proof.
+  intros A l1; induction l1 as [|a tl IH];
+    intros l2 Hnd Hincl; simpl.
+  - lia.
+  - inversion Hnd as [|a' tl' Hnotin Hndtl]; subst.
+    assert (Hin : In a l2) by (apply Hincl; left; reflexivity).
+    apply in_split in Hin as [lL [lR ->]].
+    simpl.
+    assert (Hincl' : incl tl (lL ++ lR)).
+    {
+      intros x Hx.
+      specialize (Hincl x (or_intror Hx)).
+      apply in_app_or in Hincl as [HinL|HinR].
+      - apply in_or_app. left; exact HinL.
+      - simpl in HinR. destruct HinR as [HxEq|HinR].
+        + subst. exfalso. apply Hnotin. exact Hx.
+        + apply in_or_app. right; exact HinR.
+    }
+    specialize (IH (lL ++ lR) Hndtl Hincl').
+
+    rewrite length_app in IH.
+    rewrite length_app. simpl.
+    lia.
+Qed.
+
+Lemma filter_ext_in :
+  forall (A : Type) (l : list A) (p q : A -> bool),
+    (forall x, In x l -> p x = q x) ->
+    filter p l = filter q l.
+Proof.
+  intros A l; induction l as [|a tl IH]; intros p q Hpq; simpl; auto.
+  rewrite (Hpq a (or_introl eq_refl)).
+  destruct (q a) eqn:Hqa; simpl.
+  - f_equal.
+    rewrite (IH p q (fun x Hx => Hpq x (or_intror Hx))).
+    reflexivity.
+  - rewrite (IH p q (fun x Hx => Hpq x (or_intror Hx))).
+    reflexivity.
+Qed.
+
+Lemma all_masks_length_pow2 :
+  forall n, length (all_masks n) = Nat.pow 2 n.
+Proof.
+  induction n; simpl.
+  - reflexivity.
+  - rewrite length_app.
+    repeat rewrite length_map.
+    set (k := length (all_masks n)).
+    change (k + k = 2 ^ n + (2 ^ n + 0))%nat.
+    subst k.
+    rewrite IHn.
+    lia.
+Qed.
+
+Lemma Qeq_bool_10 : Qeq_bool 1 0 = false.
+Proof. vm_compute. reflexivity. Qed.
+
+Lemma Qeq_bool_00 : Qeq_bool 0 0 = true.
+Proof. vm_compute. reflexivity. Qed.
 
 (* Count nonzero coefficients *)
 Definition support_size {n} (F : MV n) : nat :=
   length (List.filter (fun m => negb (Qeq_bool (F m) 0))
                  (all_masks n)).
+
+Lemma support_size_ext :
+  forall n (F G : MV n),
+    (forall m, F m == G m) ->
+    support_size F = support_size G.
+Proof.
+  intros n F G Heq.
+  unfold support_size.
+  apply f_equal.
+  apply filter_ext_in.
+  intros m _.
+  destruct (Qeq_bool (F m) 0) eqn:Hf;
+  destruct (Qeq_bool (G m) 0) eqn:Hg; try reflexivity.
+  - (* Hf = true, Hg = false *)
+    exfalso.
+    (* turn Hg into ~(G m == 0) *)
+    pose proof (Qeq_bool_false_neq Hg) as Hneq.
+    apply Hneq.
+    (* prove G m == 0 using Heq and Hf *)
+    apply Qeq_trans with (y := F m).
+    + apply Qeq_sym. apply Heq.
+    + apply Qeq_bool_eq. exact Hf.
+  - (* Hf = false, Hg = true *)
+    exfalso.
+    pose proof (Qeq_bool_false_neq Hf) as Hneq.
+    apply Hneq.
+    apply Qeq_trans with (y := G m).
+    + apply Heq.
+    + apply Qeq_bool_eq. exact Hg.
+Qed.
+
+        (* Support cardinality *)
+
 
 (* The support set as a list *)
 Definition support_list {n} (F : MV n) : list (Mask n) :=
@@ -151,28 +277,156 @@ Definition support_list {n} (F : MV n) : list (Mask n) :=
 Lemma support_size_le_2n : forall n (F : MV n),
   (support_size F <= Nat.pow 2 n)%nat.
 Proof.
-Admitted.
+  intros n F.
+  unfold support_size.
+  eapply Nat.le_trans.
+  - apply length_filter_le.
+  - rewrite all_masks_length_pow2.
+    lia.
+Qed.
 
 Lemma support_size_zero : forall n,
   support_size (@mv_zero n) = 0%nat.
 Proof.
-Admitted.
+  intro n.
+  unfold support_size, mv_zero.
+  rewrite Qeq_bool_00.
+  simpl.
+  induction (all_masks n); simpl; auto.
+Qed.
+
+Lemma filter_all_false_nil :
+  forall (A : Type) (p : A -> bool) (l : list A),
+    (forall x, In x l -> p x = false) ->
+    filter p l = [].
+Proof.
+  intros A p l Hall.
+  induction l as [|h t IH]; simpl; auto.
+  assert (Hp : p h = false) by (apply Hall; left; reflexivity).
+  rewrite Hp.
+  apply IH.
+  intros x Hinx.
+  apply Hall. right. exact Hinx.
+Qed.
+
+Lemma filter_singleton :
+  forall (A : Type) (p : A -> bool) (l : list A) (a : A),
+    NoDup l ->
+    In a l ->
+    p a = true ->
+    (forall x, In x l -> x <> a -> p x = false) ->
+    filter p l = [a].
+Proof.
+  intros A p l.
+  induction l as [|h t IH]; intros a Hnd Hin Hp Hall; simpl in *.
+  - contradiction.
+  - inversion Hnd as [|h' t' Hnotin Hndt]; subst.
+    simpl in Hin. destruct Hin as [Hin|Hin].
+    + subst h.
+      rewrite Hp. f_equal.
+      apply filter_all_false_nil.
+      intros x Hinx.
+      apply Hall.
+      * right; exact Hinx.
+      * intro Heq; subst x. exact (Hnotin Hinx).
+    + (* a is in tail *)
+      assert (Hha : h <> a) by (intro Heq; subst h; contradiction).
+      assert (Hph : p h = false).
+      { apply Hall; [left; reflexivity | exact Hha]. }
+      rewrite Hph.
+      apply IH.
+      * exact Hndt.
+      * exact Hin.
+      * exact Hp.
+      * intros x Hinx Hxa.
+        apply Hall; [right; exact Hinx | exact Hxa].
+Qed.
 
 Lemma support_size_basis : forall n (i : Fin.t n),
   support_size (basis (mask_single i)) = 1%nat.
 Proof.
-Admitted.
+  intros n i.
+  unfold support_size.
+  set (m0 := mask_single i).
+  set (p := fun m : Mask n => negb (Qeq_bool (basis m0 m) 0)).
+
+  assert (Hnodup : NoDup (all_masks n)) by apply all_masks_nodup.
+  assert (Hin : In m0 (all_masks n)) by apply all_masks_complete.
+
+  assert (Hp0 : p m0 = true).
+  {
+    unfold p, basis.
+    destruct (mask_eq_dec m0 m0) as [_|Hc]; [|contradiction].
+    rewrite Qeq_bool_10. reflexivity.
+  }
+
+  assert (Hall : forall x, In x (all_masks n) -> x <> m0 -> p x = false).
+  {
+    intros x Hinx Hneq.
+    unfold p, basis.
+    destruct (mask_eq_dec x m0) as [Heq|Hne].
+    - contradiction.
+    - (* basis is 0 on x, so Qeq_bool 0 0 = true, negb -> false *)
+      rewrite Qeq_bool_00. reflexivity.
+  }
+
+  (* now the filter is exactly [m0], so length is 1 *)
+  rewrite (filter_singleton (Mask n) p (all_masks n) m0 Hnodup Hin Hp0 Hall).
+  simpl. reflexivity.
+Qed.
 
 Lemma support_size_mv_one : forall n,
   support_size (@mv_one n) = 1%nat.
 Proof.
-Admitted.
+  intro n.
+  unfold mv_one, support_size.
+  set (m0 := (@mask_empty n)).
+  set (p := fun m : Mask n => negb (Qeq_bool (basis m0 m) 0)).
+
+  assert (Hnodup : NoDup (all_masks n)) by apply all_masks_nodup.
+  assert (Hin : In m0 (all_masks n)) by apply all_masks_complete.
+
+  assert (Hp0 : p m0 = true).
+  {
+    unfold p, basis.
+    destruct (mask_eq_dec m0 m0) as [_|Hc]; [|contradiction].
+    rewrite Qeq_bool_10. reflexivity.
+  }
+
+  assert (Hall : forall x, In x (all_masks n) -> x <> m0 -> p x = false).
+  {
+    intros x Hinx Hneq.
+    unfold p, basis.
+    destruct (mask_eq_dec x m0) as [Heq|Hne].
+    - contradiction.
+    - rewrite Qeq_bool_00. reflexivity.
+  }
+
+  rewrite (filter_singleton (Mask n) p (all_masks n) m0 Hnodup Hin Hp0 Hall).
+  simpl. reflexivity.
+Qed.
 
 Lemma support_size_scale : forall n (c : Q) (F : MV n),
   ~(c == 0) ->
   support_size (mv_scale c F) = support_size F.
 Proof.
-Admitted.
+  intros n c F Hc.
+  unfold support_size.
+  apply f_equal.
+  apply filter_ext_in.
+  intros m _.
+  unfold mv_scale.
+  destruct (Qeq_bool (F m) 0) eqn:Hfm.
+  - apply Qeq_bool_eq in Hfm.
+    rewrite Hfm. rewrite Qmult_0_r.
+    rewrite Qeq_bool_00. reflexivity.
+  - assert (Hnz : ~(F m == 0)) by (exact (Qeq_bool_false_neq Hfm)).
+    destruct (Qeq_bool (c * F m) 0) eqn:Hcm; try reflexivity.
+    apply Qeq_bool_eq in Hcm.
+    exfalso.
+    apply Hnz.
+    apply Qmult_integral in Hcm as [Hc0|Hf0]; [contradiction|exact Hf0].
+Qed.
 
         (* Lemma Block 2 *)
 
@@ -180,18 +434,129 @@ Admitted.
 Lemma support_size_add : forall n (F G : MV n),
   (support_size (mv_add F G) <= support_size F + support_size G)%nat.
 Proof.
-Admitted.
+  intros n F G.
+  unfold support_size.
+  set (SF := filter (fun m : Mask n => negb (Qeq_bool (F m) 0)) (all_masks n)).
+  set (SG := filter (fun m : Mask n => negb (Qeq_bool (G m) 0)) (all_masks n)).
+  set (SH := filter (fun m : Mask n => negb (Qeq_bool (mv_add F G m) 0)) (all_masks n)).
+
+  assert (Hincl : incl SH (SF ++ SG)).
+  {
+    intros m Hin.
+    apply filter_In in Hin as [HinAll Hp].
+    assert (Hsupp : supp (mv_add F G) m).
+    {
+      unfold supp.
+      destruct (Qeq_bool (mv_add F G m) 0) eqn:Heq; simpl in Hp; try discriminate.
+      apply (Qeq_bool_false_neq Heq).
+    }
+    destruct (supp_add n F G m Hsupp) as [HsF|HsG].
+    - apply in_or_app. left.
+      apply filter_In. split; [exact HinAll|].
+      destruct (Qeq_bool (F m) 0) eqn:Heq; simpl.
+      * exfalso. apply HsF. apply Qeq_bool_eq. exact Heq.
+      * reflexivity.
+    - apply in_or_app. right.
+      apply filter_In. split; [exact HinAll|].
+      destruct (Qeq_bool (G m) 0) eqn:Heq; simpl.
+      * exfalso. apply HsG. apply Qeq_bool_eq. exact Heq.
+      * reflexivity.
+  }
+
+  assert (Hnd : NoDup SH) by (apply NoDup_filter, all_masks_nodup).
+  eapply Nat.le_trans.
+  - eapply NoDup_incl_length; eauto.
+  - rewrite length_app. lia.
+Qed.
 
 (* Conv: support of F⊙G ⊆ {A⊕B : A ∈ supp(F), B ∈ supp(G)} *)
 (* So |supp(F⊙G)| ≤ |supp(F)| * |supp(G)| *)
 Lemma support_size_conv : forall n (F G : MV n),
   (support_size (mv_conv F G) <= support_size F * support_size G)%nat.
 Proof.
-Admitted.
+  intros n F G.
+  unfold support_size.
+  set (SF := filter (fun m : Mask n => negb (Qeq_bool (F m) 0)) (all_masks n)).
+  set (SG := filter (fun m : Mask n => negb (Qeq_bool (G m) 0)) (all_masks n)).
+  set (SH := filter (fun m : Mask n => negb (Qeq_bool (mv_conv F G m) 0)) (all_masks n)).
+
+  (* all xor-combinations of support lists *)
+  set (xor_sumset :=
+    concat (map (fun A => map (fun B => mask_xor A B) SG) SF)).
+
+  (* length of the xor_sumset list is |SF| * |SG| *)
+  assert (Hlen : length xor_sumset = (length SF * length SG)%nat).
+  {
+    unfold xor_sumset.
+    induction SF as [|A tl IH]; simpl.
+    - lia.
+    - rewrite length_app, length_map, IH. lia.
+  }
+
+  (* SH ⊆ xor_sumset *)
+  assert (Hincl : incl SH xor_sumset).
+  {
+    intros U HinU.
+    apply filter_In in HinU as [HinAll HpU].
+    assert (Hsupp : supp (mv_conv F G) U).
+    {
+      unfold supp.
+      destruct (Qeq_bool (mv_conv F G U) 0) eqn:Heq; simpl in HpU; try discriminate.
+      apply (Qeq_bool_false_neq Heq).
+    }
+    destruct (support_conv_subset_xor n F G U Hsupp)
+      as [A [B [HsA [HsB Hxor]]]].
+    subst U.
+
+    assert (HinA : In A SF).
+    {
+      unfold SF.
+      apply filter_In. split.
+      - apply all_masks_complete.
+      - destruct (Qeq_bool (F A) 0) eqn:Heq; simpl.
+        + exfalso. apply HsA. apply Qeq_bool_eq. exact Heq.
+        + reflexivity.
+    }
+    assert (HinB : In B SG).
+    {
+      unfold SG.
+      apply filter_In. split.
+      - apply all_masks_complete.
+      - destruct (Qeq_bool (G B) 0) eqn:Heq; simpl.
+        + exfalso. apply HsB. apply Qeq_bool_eq. exact Heq.
+        + reflexivity.
+    }
+
+    unfold xor_sumset.
+    apply in_concat.
+    exists (map (fun B0 : Mask n => mask_xor A B0) SG).
+    split.
+    - apply in_map_iff. exists A. split; [reflexivity | exact HinA].
+    - apply in_map. exact HinB.
+  }
+
+  assert (Hnd : NoDup SH) by (apply NoDup_filter, all_masks_nodup).
+  eapply Nat.le_trans.
+  - eapply NoDup_incl_length; eauto.
+  - rewrite Hlen. unfold SF, SG.
+    lia.
+Qed.
 
         (* Lemma Block 3 *)
 
 (* Static support size bound from expression structure *)
+
+(*
+OLD support_size_bound
+Fixpoint support_size_bound {n} (e : GA_expr n) : nat :=
+  match e with
+  | Basis _    => 1
+  | Scalar _   => 1
+  | Cln_Grade.Add e1 e2  => support_size_bound e1 + support_size_bound e2
+  | Mul _ _    => Nat.pow 2 n  (* worst case; keeps Block 3 mechanical *)
+  | Conv e1 e2 => support_size_bound e1 * support_size_bound e2
+  end.
+*)
 Fixpoint support_size_bound {n} (e : GA_expr n) : nat :=
   match e with
   | Basis _    => 1
@@ -201,16 +566,215 @@ Fixpoint support_size_bound {n} (e : GA_expr n) : nat :=
       match e1, e2 with
       | Scalar _, _ => support_size_bound e2
       | _, Scalar _ => support_size_bound e1
-      | _, _        => Nat.pow 2 n  (* worst case *)
+      | _, _        => Nat.pow 2 n
       end
   | Conv e1 e2 => support_size_bound e1 * support_size_bound e2
   end.
+
+Lemma eval_mul_scalar_l :
+  forall n (sq : Vector.t Q n) (q : Q) (e : GA_expr n),
+    forall m,
+      eval_expr sq (Mul (Scalar q) e) m
+      ==
+      mv_scale q (eval_expr sq e) m.
+Proof.
+  intros n sq q e m.
+  simpl.  (* eval_expr Mul / Scalar *)
+  rewrite (@mv_gp_scale_l n sq q (@mv_one n) (eval_expr sq e) m).
+  unfold mv_scale.
+  rewrite (@mv_gp_one_l n sq (eval_expr sq e) m).
+  ring.
+Qed.
+
+Lemma eval_mul_scalar_r :
+  forall n (sq : Vector.t Q n) (q : Q) (e : GA_expr n),
+    forall m,
+      eval_expr sq (Mul e (Scalar q)) m
+      ==
+      mv_scale q (eval_expr sq e) m.
+Proof.
+  intros n sq q e m.
+  simpl.
+  rewrite (@mv_gp_scale_r n sq q (eval_expr sq e) (@mv_one n) m).
+  unfold mv_scale.
+  rewrite (@mv_gp_one_r n sq (eval_expr sq e) m).
+  ring.
+Qed.
 
 Theorem eval_support_size_le :
   forall n (sq : Vector.t Q n) (e : GA_expr n),
     (support_size (eval_expr sq e) <= support_size_bound e)%nat.
 Proof.
-Admitted.
+  intros n sq e.
+  induction e as [i|c|e1 IH1 e2 IH2|e1 IH1 e2 IH2|e1 IH1 e2 IH2]; simpl.
+  - (* Basis *)
+    rewrite support_size_basis. lia.
+
+  - (* Scalar *)
+    destruct (Qeq_dec c 0) as [Hc0|Hc0].
+    + (* c = 0 *)
+      assert (He : forall m, mv_scale c (@mv_one n) m == (@mv_zero n) m).
+      { intro m. unfold mv_scale, mv_zero. rewrite Hc0. ring. }
+      rewrite (support_size_ext n (mv_scale c (@mv_one n)) (@mv_zero n) He).
+      rewrite support_size_zero. lia.
+    + (* c <> 0 *)
+      rewrite (support_size_scale n c (@mv_one n) Hc0).
+      rewrite support_size_mv_one. lia.
+
+  - (* Add *)
+    eapply Nat.le_trans.
+    + apply support_size_add.
+    + lia.
+
+  - (* Mul *)
+    (* Do NOT simpl here; we want eval_expr (Mul ...) to remain visible for rewrites. *)
+    destruct e1 as [i1|q1|a1 b1|a1 b1|a1 b1];
+    destruct e2 as [i2|q2|a2 b2|a2 b2|a2 b2].
+
+    + (* Basis * Basis *)
+      simpl. eapply Nat.le_trans; [apply support_size_le_2n | lia].
+
+    + (* Basis * Scalar *)
+      change (eval_expr sq (Basis i1) ⋆ eval_expr sq (Scalar q2))
+        with (eval_expr sq (Mul (Basis i1) (Scalar q2))).
+      rewrite (support_size_ext n
+                (eval_expr sq (Mul (Basis i1) (Scalar q2)))
+                (mv_scale q2 (eval_expr sq (Basis i1)))
+                (eval_mul_scalar_r n sq q2 (Basis i1))).
+      destruct (Qeq_dec q2 0) as [Hq0|Hq0].
+      * assert (Hz : forall m, mv_scale q2 (eval_expr sq (Basis i1)) m == (@mv_zero n) m).
+        { intro m. unfold mv_scale, mv_zero. rewrite Hq0. ring. }
+        rewrite (support_size_ext n (mv_scale q2 (eval_expr sq (Basis i1))) (@mv_zero n) Hz).
+        rewrite support_size_zero. simpl. lia.
+      * rewrite (support_size_scale n q2 (eval_expr sq (Basis i1)) Hq0).
+        simpl. exact IH1.
+
+    + (* Basis * Add *)
+      simpl. eapply Nat.le_trans; [apply support_size_le_2n | lia].
+
+    + (* Basis * Mul *)
+      simpl. eapply Nat.le_trans; [apply support_size_le_2n | lia].
+
+    + (* Basis * Conv *)
+      simpl. eapply Nat.le_trans; [apply support_size_le_2n | lia].
+
+    + (* Scalar * Basis *)
+      change (eval_expr sq (Scalar q1) ⋆ eval_expr sq (Basis i2))
+        with (eval_expr sq (Mul (Scalar q1) (Basis i2))).
+      rewrite (support_size_ext n
+                (eval_expr sq (Mul (Scalar q1) (Basis i2)))
+                (mv_scale q1 (eval_expr sq (Basis i2)))
+                (eval_mul_scalar_l n sq q1 (Basis i2))).
+      destruct (Qeq_dec q1 0) as [Hq0|Hq0].
+      * assert (Hz : forall m, mv_scale q1 (eval_expr sq (Basis i2)) m == (@mv_zero n) m).
+        { intro m. unfold mv_scale, mv_zero. rewrite Hq0. ring. }
+        rewrite (support_size_ext n (mv_scale q1 (eval_expr sq (Basis i2))) (@mv_zero n) Hz).
+        rewrite support_size_zero. simpl. lia.
+      * rewrite (support_size_scale n q1 (eval_expr sq (Basis i2)) Hq0).
+        simpl. exact IH2.
+    
+    + (* Scalar * Scalar *)
+      change (eval_expr sq (Scalar q1) ⋆ eval_expr sq (Scalar q2))
+        with (eval_expr sq (Mul (Scalar q1) (Scalar q2))).
+      rewrite (support_size_ext n
+                (eval_expr sq (Mul (Scalar q1) (Scalar q2)))
+                (mv_scale q1 (eval_expr sq (Scalar q2)))
+                (eval_mul_scalar_l n sq q1 (Scalar q2))).
+      destruct (Qeq_dec q1 0) as [Hq0|Hq0].
+      * assert (Hz : forall m, mv_scale q1 (eval_expr sq (Scalar q2)) m == (@mv_zero n) m).
+        { intro m. unfold mv_scale, mv_zero. rewrite Hq0. ring. }
+        rewrite (support_size_ext n (mv_scale q1 (eval_expr sq (Scalar q2))) (@mv_zero n) Hz).
+        rewrite support_size_zero. simpl. lia.
+      * rewrite (support_size_scale n q1 (eval_expr sq (Scalar q2)) Hq0).
+        simpl. exact IH2.
+
+    + (* Scalar * Add *)
+      change (eval_expr sq (Scalar q1) ⋆ eval_expr sq (Cln_Grade.Add a2 b2))
+        with (eval_expr sq (Mul (Scalar q1) (Cln_Grade.Add a2 b2))).
+      rewrite (support_size_ext n
+                (eval_expr sq (Mul (Scalar q1) (Cln_Grade.Add a2 b2)))
+                (mv_scale q1 (eval_expr sq (Cln_Grade.Add a2 b2)))
+                (eval_mul_scalar_l n sq q1 (Cln_Grade.Add a2 b2))).
+      destruct (Qeq_dec q1 0) as [Hq0|Hq0].
+      * assert (Hz : forall m, mv_scale q1 (eval_expr sq (Cln_Grade.Add a2 b2)) m == (@mv_zero n) m).
+        { intro m. unfold mv_scale, mv_zero. rewrite Hq0. ring. }
+        rewrite (support_size_ext n (mv_scale q1 (eval_expr sq (Cln_Grade.Add a2 b2))) (@mv_zero n) Hz).
+        rewrite support_size_zero. simpl. lia.
+      * rewrite (support_size_scale n q1 (eval_expr sq (Cln_Grade.Add a2 b2)) Hq0).
+        simpl. exact IH2.
+
+    + (* Scalar * Mul *)
+      change (eval_expr sq (Scalar q1) ⋆ eval_expr sq (Mul a2 b2))
+        with (eval_expr sq (Mul (Scalar q1) (Mul a2 b2))).
+      rewrite (support_size_ext n
+                (eval_expr sq (Mul (Scalar q1) (Mul a2 b2)))
+                (mv_scale q1 (eval_expr sq (Mul a2 b2)))
+                (eval_mul_scalar_l n sq q1 (Mul a2 b2))).
+      destruct (Qeq_dec q1 0) as [Hq0|Hq0].
+      * assert (Hz : forall m, mv_scale q1 (eval_expr sq (Mul a2 b2)) m == (@mv_zero n) m).
+        { intro m. unfold mv_scale, mv_zero. rewrite Hq0. ring. }
+        rewrite (support_size_ext n (mv_scale q1 (eval_expr sq (Mul a2 b2))) (@mv_zero n) Hz).
+        rewrite support_size_zero. simpl. lia.
+      * rewrite (support_size_scale n q1 (eval_expr sq (Mul a2 b2)) Hq0).
+        simpl. exact IH2.
+
+    + (* Scalar * Conv *)
+      change (eval_expr sq (Scalar q1) ⋆ eval_expr sq (Conv a2 b2))
+        with (eval_expr sq (Mul (Scalar q1) (Conv a2 b2))).
+      rewrite (support_size_ext n
+                (eval_expr sq (Mul (Scalar q1) (Conv a2 b2)))
+                (mv_scale q1 (eval_expr sq (Conv a2 b2)))
+                (eval_mul_scalar_l n sq q1 (Conv a2 b2))).
+      destruct (Qeq_dec q1 0) as [Hq0|Hq0].
+      * assert (Hz : forall m, mv_scale q1 (eval_expr sq (Conv a2 b2)) m == (@mv_zero n) m).
+        { intro m. unfold mv_scale, mv_zero. rewrite Hq0. ring. }
+        rewrite (support_size_ext n (mv_scale q1 (eval_expr sq (Conv a2 b2))) (@mv_zero n) Hz).
+        rewrite support_size_zero. simpl. lia.
+      * rewrite (support_size_scale n q1 (eval_expr sq (Conv a2 b2)) Hq0).
+        simpl. exact IH2.
+
+    (* remaining cases: neither side is Scalar => crude 2^n bound *)
+    all: (simpl; eapply Nat.le_trans; [apply support_size_le_2n | lia]).
+
+  + (* Conv *)
+    eapply Nat.le_trans.
+    * apply support_size_conv.
+    * nia.
+Qed.
+
+
+
+Theorem eval_support_size_le :
+  forall n (sq : Vector.t Q n) (e : GA_expr n),
+    (support_size (eval_expr sq e) <= support_size_bound e)%nat.
+Proof.
+  intros n sq e.
+  induction e as [i|c|e1 IH1 e2 IH2|e1 IH1 e2 IH2|e1 IH1 e2 IH2]; simpl.
+  - (* Basis *)
+    rewrite support_size_basis. lia.
+  - (* Scalar *)
+    destruct (Qeq_dec c 0) as [Hc0|Hc0].
+    + (* zero scalar *)
+      assert (He : forall m, mv_scale c (@mv_one n) m == (@mv_zero n) m).
+      { intro m. unfold mv_scale, mv_zero. rewrite Hc0. ring. }
+      rewrite (support_size_ext n (mv_scale c mv_one) mv_zero He).
+      rewrite support_size_zero. lia.
+    + (* nonzero scalar *)
+      rewrite (support_size_scale n c mv_one Hc0).
+      rewrite support_size_mv_one. lia.
+  - (* Add *)
+    eapply Nat.le_trans.
+    + apply support_size_add.
+    + lia.
+  - (* Mul: crude bound by 2^n *)
+    eapply Nat.le_trans.
+    + apply support_size_le_2n.
+    + lia.
+  - (* Conv *)
+    eapply Nat.le_trans.
+    + apply support_size_conv.
+    + nia.
+Qed.
 
         (* Lemma Block 4 *)
 
